gwhrnbgw

Games/games/Chomp_work.lean
@@ -29,17 +29,21 @@ instance : DecidableRel nondomi :=
   rw [nondomi]
   exact Not.decidable
 
-instance (l : List (ℕ × ℕ)) : DecidablePred (fun p => ∀ q ∈ l, nondomi q p) :=
+instance (ini : Finset (ℕ × ℕ)) (l : List (ℕ × ℕ)) : DecidablePred (fun p => ∀ q ∈ l, q ∈ ini → nondomi q p) :=
   by
   intro p
   dsimp [nondomi,domi]
-  exact List.decidableBAll (fun x => ¬(x.1 ≤ p.1 ∧ x.2 ≤ p.2)) l
+  exact List.decidableBAll (fun x => x ∈ ini → ¬(x.1 ≤ p.1 ∧ x.2 ≤ p.2)) l
 
-
+lemma domi_trans {p q r: ℕ × ℕ} : domi p q → domi q r → domi p r :=
+  by
+  intro a b
+  dsimp [domi] at *
+  exact ⟨ le_trans a.1 b.1, le_trans a.2 b.2⟩
 
 
 def Chomp_state (ini : Finset (ℕ × ℕ)) (hist : List (ℕ × ℕ)) :=
-  ini.filter (fun p => ∀ q ∈ hist, nondomi q p)
+  ini.filter (fun p => ∀ q ∈ hist, q ∈ ini → nondomi q p)
 
 
 lemma Chomp_state_sub (ini : Finset (ℕ × ℕ)) (l L :  List (ℕ × ℕ)) :
@@ -79,11 +83,20 @@ lemma Chomp_state_blind (ini : Finset (ℕ × ℕ)) (hist prehist : List (ℕ ×
     simp_rw [Finset.mem_filter] at *
     constructor
     · exact H.1.1
-    · intro q qq
+    · intro q qq qi
       rw [List.mem_append] at qq
       cases' qq with k k
-      · exact H.2 q k
-      · exact H.1.2 q k
+      · by_cases C : ∀ q_1 ∈ prehist, q_1 ∈ ini → nondomi q_1 q
+        · exact H.2 q k ⟨qi, C⟩
+        · push_neg at C
+          obtain ⟨q',q'pre,q'ini, no⟩ := C
+          have := H.1.2 q' q'pre q'ini
+          dsimp [nondomi] at *
+          rw [not_not] at no
+          intro con
+          apply this
+          exact domi_trans no con
+      · exact H.1.2 q k qi
   · intro H
     dsimp [Chomp_state] at *
     simp_rw [Finset.mem_filter] at *
@@ -93,8 +106,8 @@ lemma Chomp_state_blind (ini : Finset (ℕ × ℕ)) (hist prehist : List (ℕ ×
       · intro q qh
         apply H.2
         exact List.mem_append_right hist qh
-    · intro q qh
-      apply H.2
+    · intro q qh ⟨qi, _⟩
+      apply H.2 _ _ qi
       exact List.mem_append.mpr (Or.inl qh)
 
 
@@ -123,7 +136,7 @@ lemma Chomp_state_ini_zero (hist : List (ℕ × ℕ)) (hh : (0,0) ∉ hist): Cho
   by
   dsimp [Chomp_state]
   rw [Finset.filter_eq_self]
-  intro x xdef q qh
+  intro x xdef q qh qi
   rw [Finset.mem_singleton] at xdef
   rw [xdef]
   dsimp [nondomi, domi]
@@ -144,14 +157,14 @@ lemma Chomp_state_has_zero_iff_hist_has_zero
     rw [Finset.mem_filter] at c
     dsimp [nondomi, domi] at c
     intro con
-    apply c.2 _ con
+    apply c.2 _ con c.1
     decide
   · intro c
     dsimp [Chomp_state]
     rw [Finset.mem_filter]
     constructor
     · exact hini
-    · intro q qh
+    · intro q qh qi
       dsimp [nondomi, domi]
       intro con
       simp_all only [nonpos_iff_eq_zero]
@@ -159,16 +172,16 @@ lemma Chomp_state_has_zero_iff_hist_has_zero
       simp_all only
 
 lemma Chomp_state_sub_ini (ini : Finset (ℕ × ℕ) ) (hist : List (ℕ × ℕ)) :
-  Chomp_state ini hist ⊆ ini := by dsimp [Chomp_state]; exact Finset.filter_subset (fun p => ∀ q ∈ hist, nondomi q p) ini
+  Chomp_state ini hist ⊆ ini := by dsimp [Chomp_state]; exact Finset.filter_subset (fun p => ∀ q ∈ hist, q ∈ ini → nondomi q p) ini
 
-lemma Chomp_state_hist_zero (ini : Finset (ℕ × ℕ) ) (hist : List (ℕ × ℕ)) (main : (0,0) ∈ hist) :
+lemma Chomp_state_hist_zero (ini : Finset (ℕ × ℕ) ) (hini : (0,0) ∈ ini) (hist : List (ℕ × ℕ)) (main : (0,0) ∈ hist) :
   Chomp_state ini hist = ∅ :=
   by
   rw [Finset.eq_empty_iff_forall_not_mem]
   intro x xdef
   dsimp [Chomp_state] at xdef
   rw [Finset.mem_filter] at xdef
-  apply xdef.2 _ main
+  apply xdef.2 _ main hini
   dsimp [domi]
   simp_all only [Prod.forall, zero_le, and_self]
 
@@ -181,7 +194,7 @@ lemma Chomp_state_state_empty (ini : Finset (ℕ × ℕ) ) (hini : (0,0) ∈ ini
   dsimp [nondomi, domi] at main
   push_neg at main
   specialize main _ hini
-  obtain ⟨q, qh, qz1, qz2⟩ := main
+  obtain ⟨q, qh, _, qz1, qz2⟩ := main
   simp only [nonpos_iff_eq_zero] at *
   convert qh <;> {rw [eq_comm] ; assumption}
 
@@ -197,13 +210,13 @@ lemma Chomp_state_state_empty (ini : Finset (ℕ × ℕ) ) (hini : (0,0) ∈ ini
 --   · exact leg.nd
 
 
-lemma Chomp_law_sub (ini : Finset (ℕ × ℕ) ) (l L : List (ℕ × ℕ)) (act : ℕ × ℕ) (leg : Chomp_law ini (l ++ L) act) :
-  Chomp_law ini L act :=
-  by
-  refine' ⟨leg.act_mem, _ , leg.nz_act⟩
-  intro q qdef
-  apply leg.nd
-  exact List.mem_append_right l qdef
+-- lemma Chomp_law_sub (ini : Finset (ℕ × ℕ) ) (l L : List (ℕ × ℕ)) (act : ℕ × ℕ) (leg : Chomp_law ini (l ++ L) act) :
+--   Chomp_law ini L act :=
+--   by
+--   refine' ⟨leg.act_mem, _ , leg.nz_act⟩
+--   intro q qdef
+--   apply leg.nd
+--   exact List.mem_append_right l qdef
 
 
 
@@ -254,7 +267,7 @@ lemma preChomp_law_careless (height length : ℕ) :
                           · intro e eh
                             apply c.nd
                             exact List.mem_append_right hist eh
-                        · intro e eh
+                        · intro e eh ei
                           apply c.nd
                           exact List.mem_append_left prehist eh
                         · apply c.nz_act
